More useful word theorems

opentheory/examples/all.ml
@@ -4,13 +4,11 @@
 
 start_logging ();;
 
-loads "opentheory/examples/parser.ml";;
 loads "opentheory/examples/modular.ml";;
 loads "opentheory/examples/word.ml";;
 loads "opentheory/examples/byte.ml";;
 loads "opentheory/examples/word16.ml";;
-(***
+loads "opentheory/examples/parser.ml";;
 loads "opentheory/examples/char.ml";;
-***)
 
 stop_logging ();;
